ROOT
@@ -19,7 +19,8 @@ session Propagation_Extras in propagation_extras = Progress_Tracking +
 (*     Executable
     Termination *)
 
-session Dataplane in dataplane = Nondeterministic_Dataflow + 
+session 
+Dataplane in dataplane = Nondeterministic_Dataflow + 
   options [timeout = 6000]
   sessions
     DFS_Framework
